replaced notation, reordered, sectionning ... + display of the main results for the encoding

hfs.v
@@ -16,32 +16,62 @@ Set Implicit Arguments.
 Section btree.
 
   Reserved Notation "⌞ x ⌟" (at level 0).
-  Reserved Notation "x ∙ y" (at level 2, right associativity).
+  Reserved Notation "x ∙ y"  (at level 2, right associativity).
+  Reserved Notation "x ⪧ y" (at level 2, right associativity).
   Reserved Notation "x ≈ y" (at level 70, no associativity).
   Reserved Notation "x ≉ y" (at level 70, no associativity).
   Reserved Notation "x ≾ y" (at level 70, no associativity).
-  Reserved Notation "x ∊ y" (at level 70, no associativity).
+  Reserved Notation "x ∈ y" (at level 70, no associativity).
+  Reserved Notation "x ∉ y" (at level 70, no associativity).
   Reserved Notation "x ⋷ y" (at level 70, no associativity).
   Reserved Notation "x ≺ y" (at level 70, no associativity).
+  Reserved Notation "x ∪ y" (at level 61, left associativity).
 
-  (* ⌞ ⌟ ε ∙ ≈ ≉ ∊ ⋷  ≾ ≺ *)
+  (* ⌞ ⌟ ∅ ⪧ ≈ ≉ ∈ ∉ ⋷  ≾ ≺ ε ∙*)
 
   Inductive bt : Set := bt_leaf | bt_node : bt -> bt -> bt.
 
-  Notation ε := bt_leaf.
-  Infix "∙" := bt_node.
+  Notation "∅" := bt_leaf.
 
+  Infix "∙" := bt_node.  (* replaced with a non symmetric notation *)
+  Infix "⪧" := bt_node.
+
+  (** Indeed x⪧t represent {x}∪t *)
+
+  Section bt_rect'.
+
+    (** When we inspect bt as lists, we can switch to this principle 
+
+        In fact, btrees code HF-sets like this
+
+            {x1,...,xn} = x1⪧...⪧xn⪧∅
+
+        We could also use rose-trees but may be this would be more
+        difficult ?
+     *)
+
+    Variables (P : bt -> Type) 
+              (HP0 : P ∅)
+              (HP1 : forall x t, P t -> P (x⪧t)).
+  
+    Theorem bt_rect' t : P t.
+    Proof. induction t; auto. Qed.
+
+  End bt_rect'.
+   
   Fact bt_eq_dec (s t : bt) : { s = t } + { s <> t }.
   Proof. decide equality. Qed.
 
   Fixpoint bt_depth t :=
     match t with
-      | ε   => 0
-      | r∙s => max (S ⌞r⌟) ⌞s⌟
+      | ∅   => 0
+      | r⪧s => max (S ⌞r⌟) ⌞s⌟
     end
   where "⌞ t ⌟" := (bt_depth t).
 
-  (* ⌞ ⌟ ε ∙ ≈ *)
+  Print bt_depth.
+
+  (* ⌞ ⌟ ∅ ⪧ ≈ *)
 
   Inductive bt_equiv : bt -> bt -> Prop :=
     | in_bte_refl : forall s,             s ≈ s
@@ -50,31 +80,33 @@ Section btree.
     | in_bte_tran : forall r s t,         r ≈ s
                                        -> s ≈ t
                                        -> r ≈ t
-    | in_bte_cntr : forall s t,       s∙s∙t ≈ s∙t
-    | in_bte_comm : forall s t u,     s∙t∙u ≈ t∙s∙u
+    | in_bte_cntr : forall s t,       s⪧s⪧t ≈ s⪧t
+    | in_bte_comm : forall s t u,     s⪧t⪧u ≈ t⪧s⪧u
     | in_bte_cngr : forall s s' t t',     s ≈ s'
                                        -> t ≈ t'
-                                   ->   s∙t ≈ s'∙t'
+                                   ->   s⪧t ≈ s'⪧t'
   where "s ≈ t" := (bt_equiv s t).
 
+  Notation bte_refl := in_bte_refl.
   Notation bte_trans := in_bte_tran.
  
   Hint Constructors bt_equiv.
 
+  Fact bte_sym x y : x ≈ y <-> y ≈ x.
+  Proof. split; auto. Qed.
+
   Notation "s ≉ t" := (~ s ≈ t).
 
-  Fact bte_leaf_eq s t : s ≈ t -> (s = ε <-> t = ε).
-  Proof.
-    induction 1; try tauto; split; discriminate.
-  Qed.
+  Fact bte_leaf_eq s t : s ≈ t -> (s = ∅ <-> t = ∅).
+  Proof. induction 1; try tauto; split; discriminate. Qed.
 
-  Fact bte_discr s t : s∙t ≉ ε.
+  Fact bte_discr s t : s⪧t ≉ ∅.
   Proof. 
    intros H; apply bte_leaf_eq in H.
    generalize (proj2 H eq_refl); discriminate.
   Qed.
 
-  Fact bte_inv_0 s : s ≈ ε <-> s = ε.
+  Fact bte_inv_0 s : s ≈ ∅ <-> s = ∅.
   Proof.
     split.
     + intros H; destruct s; auto.
@@ -82,397 +114,493 @@ Section btree.
     + intros ->; auto.
   Qed.
 
-  Notation "s ∊ t" := (s∙t ≈ t).
+  Notation "s ∈ t" := (s⪧t ≈ t).
+  Notation "s ∉ t" := (~ s ∈ t).
 
-  (* ⌞ ⌟ ε ∙ ≈  ∊ ⋷  *)
+  (* ⌞ ⌟ ∅ ⪧ ≈  ∈ ⋷  *)
 
-  Inductive bt_restr_mem : bt -> bt -> Prop :=
-    | in_btrm_0 : forall s t,    s ⋷ s∙t
-    | in_btrm_1 : forall s t u,  s ⋷ u
-                             ->  s ⋷ t∙u
-  where "s ⋷ t" := (bt_restr_mem s t).
+  Section establishing_membership_inversion.
 
-  Hint Constructors bt_restr_mem.
+    Inductive bt_restr_mem : bt -> bt -> Prop :=
+      | in_btrm_0 : forall s t,    s ⋷ s⪧t
+      | in_btrm_1 : forall s t u,  s ⋷ u
+                               ->  s ⋷ t⪧u
+    where "s ⋷ t" := (bt_restr_mem s t).
 
-  Fact btrm_inv u s t : u ⋷ s∙t <-> u = s \/ u ⋷ t.
-  Proof.
-    split.
-    + inversion 1; auto.
-    + intros [ <- | ]; constructor; auto.
-  Qed.
+    Hint Constructors bt_restr_mem.
 
-  Notation "s ≾ t" := (forall u, u ⋷ s -> exists v, v ⋷ t /\ u ≈ v).
+    Fact btrm_inv u s t : u ⋷ s⪧t <-> u = s \/ u ⋷ t.
+    Proof.
+      split.
+      + inversion 1; auto.
+      + intros [ <- | ]; constructor; auto.
+    Qed.
 
-  Fact bt_rincl_refl s : s ≾ s.
-  Proof. intros u; exists u; auto. Qed.
+    Notation "s ≾ t" := (forall u, u ⋷ s -> exists v, v ⋷ t /\ u ≈ v).
 
-  Fact bt_rincl_trans r s t : r ≾ s -> s ≾ t -> r ≾ t.
-  Proof.
-    intros H1 H2 u Hu.
-    destruct H1 with (1 := Hu) as (v & Hv & H3).
-    destruct H2 with (1 := Hv) as (w & ? & ?).
-    exists w; split; auto.
-    apply bte_trans with v; auto.
-  Qed.
+    Fact bt_rincl_refl s : s ≾ s.
+    Proof. intros u; exists u; auto. Qed.
 
-  Hint Resolve bt_rincl_refl bt_rincl_trans.
+    Fact bt_rincl_trans r s t : r ≾ s -> s ≾ t -> r ≾ t.
+    Proof.
+      intros H1 H2 u Hu.
+      destruct H1 with (1 := Hu) as (v & Hv & H3).
+      destruct H2 with (1 := Hv) as (w & ? & ?).
+      exists w; split; auto.
+      apply bte_trans with v; auto.
+    Qed.
 
-  Lemma bte_rincl s t : s ≈ t -> s ≾ t.
-  Proof.
-    intros H.
-    assert (s ≾ t /\ t ≾ s) as K; [ | apply K ].
-    induction H as [ s | s t H IH | r s t H1 [] H2 [] | s t | s t u | s s' t t' H1 [H2 H3] H4 [H5 H6] ]; auto; try tauto.
-    + split; apply bt_rincl_trans with s; auto.
-    + split; intros u; rewrite btrm_inv; intros [ <- | ]; exists u; auto.
-    + split; intros v; rewrite btrm_inv; intros [ <- | ]; exists v; auto;
-        revert H; rewrite btrm_inv; intros [ <- | ]; auto.
-    + split.
-      * intros u; rewrite btrm_inv.
-        intros [ <- | ].
-        - exists s'; auto.
-        - destruct (H5 _ H) as (v & ? & ?); exists v; auto.
-      * intros u; rewrite btrm_inv.
-        intros [ <- | ].
-        - exists s; auto.
-        - destruct (H6 _ H) as (v & ? & ?); exists v; auto.
-  Qed.
+    Hint Resolve bt_rincl_refl bt_rincl_trans.
+
+    Lemma bte_rincl s t : s ≈ t -> s ≾ t.
+    Proof.
+      intros H.
+      assert (s ≾ t /\ t ≾ s) as K; [ | apply K ].
+      induction H as [ s | s t H IH | r s t H1 [] H2 [] 
+                     | s t | s t u | s s' t t' H1 [H2 H3] H4 [H5 H6] ]; 
+        auto; try tauto.
+      + split; apply bt_rincl_trans with s; auto.
+      + split; intros u; rewrite btrm_inv; intros [ <- | ]; exists u; auto.
+      + split; intros v; rewrite btrm_inv; intros [ <- | ]; exists v; auto;
+          revert H; rewrite btrm_inv; intros [ <- | ]; auto.
+      + split.
+        * intros u; rewrite btrm_inv.
+          intros [ <- | ].
+          - exists s'; auto.
+          - destruct (H5 _ H) as (v & ? & ?); exists v; auto.
+        * intros u; rewrite btrm_inv.
+          intros [ <- | ].
+          - exists s; auto.
+          - destruct (H6 _ H) as (v & ? & ?); exists v; auto.
+    Qed.
  
-  Fact btrm_btm s t : s ⋷ t -> s ∊ t.
-  Proof.
-    induction 1 as [ | s t u ]; try (constructor; auto; fail).
-    constructor; apply bte_trans with (t∙s∙u); auto.
-  Qed.
+    Fact btrm_btm s t : s ⋷ t -> s ∈ t.
+    Proof.
+      induction 1 as [ | s t u ]; try (constructor; auto; fail).
+      constructor; apply bte_trans with (t⪧s⪧u); auto.
+    Qed.
 
-  Hint Resolve btrm_btm.
+    Hint Resolve btrm_btm.
 
-  Fact btm_congr_l s t u : s ≈ t -> s ∊ u -> t ∊ u.
-  Proof.
-    intros H1 H2.
-    apply bte_trans with (2 := H2); auto.
-  Qed.
+    Fact btm_congr_l s t u : s ≈ t -> s ∈ u -> t ∈ u.
+    Proof.
+      intros H1 H2.
+      apply bte_trans with (2 := H2); auto.
+    Qed.
 
-  Fact btm_congr_r s t u : s ≈ t -> u ∊ s -> u ∊ t.
-  Proof.
-    intros H1 H2.
-    apply bte_trans with (2 := H1),
-          bte_trans with (2 := H2); auto.
-  Qed.
+    Fact btm_congr_r s t u : s ≈ t -> u ∈ s -> u ∈ t.
+    Proof.
+      intros H1 H2.
+      apply bte_trans with (2 := H1),
+            bte_trans with (2 := H2); auto.
+    Qed.
 
-  Fact btm_inv_0 s : s ∊ ε <-> False.
-  Proof. split; try tauto; apply bte_discr. Qed.
+    Fact btm_inv_0 s : s ∈ ∅ <-> False.
+    Proof. split; try tauto; apply bte_discr. Qed.
 
-  Fact btm_inv u s t : u ∊ s∙t <-> u ≈ s \/ u ∊ t.
-  Proof.
-    split.
-    + intros H.
-      destruct (@bte_rincl _ _ H u) as (v & H1 & ?); auto.
-      revert H1; rewrite btrm_inv; intros [ <- | ]; auto.
-      right; apply bte_trans with (v∙t); auto.
-    + intros [ H | H ].
-      * apply btm_congr_l with s; auto.
-      * apply bte_trans with (1 := in_bte_comm _ _ _); auto.
-  Qed.
+    Fact btm_inv u s t : u ∈ s⪧t <-> u ≈ s \/ u ∈ t.
+    Proof.
+      split.
+      + intros H.
+        destruct (@bte_rincl _ _ H u) as (v & H1 & ?); auto.
+        revert H1; rewrite btrm_inv; intros [ <- | ]; auto.
+        right; apply bte_trans with (v⪧t); auto.
+      + intros [ H | H ].
+        * apply btm_congr_l with s; auto.
+        * apply bte_trans with (1 := in_bte_comm _ _ _); auto.
+    Qed.
 
-  Inductive bt_lt : bt -> bt -> Prop :=
-    | in_btlt_0 : forall s t,                   ε ≺ s∙t 
-    | in_btlt_1 : forall s s' t t', s ≺ s' -> s∙t ≺ s'∙t'
-    | in_btlt_2 : forall s t t',    t ≺ t' -> s∙t ≺ s∙t'
-  where "s ≺ t" := (bt_lt s t).
+  End establishing_membership_inversion.
 
-  Hint Constructors bt_lt.
+  Section establishing_decidability.
 
-  Fact bt_lt_inv s t : s ≺ t -> s = ε /\ (exists u v, t = u∙v)
-                             \/ (exists u u' v v', s = u∙v /\ t = u'∙v' /\ u ≺ u')
-                             \/ (exists u v v', s = u∙v /\ t = u∙v' /\ v ≺ v').
-  Proof.
-    destruct 1.
-    + left; split; auto; exists s, t; auto.
-    + right; left; exists s, s', t, t'; auto.
-    + do 2 right; exists s, t, t'; auto.
-  Qed.
+    Inductive bt_lt : bt -> bt -> Prop :=
+      | in_btlt_0 : forall s t,                   ∅ ≺ s⪧t 
+      | in_btlt_1 : forall s s' t t', s ≺ s' -> s⪧t ≺ s'⪧t'
+      | in_btlt_2 : forall s t t',    t ≺ t' -> s⪧t ≺ s⪧t'
+    where "s ≺ t" := (bt_lt s t).
 
-  Fact bt_lt_node_inv s t u : s∙t ≺ u -> (exists s' t', u = s'∙t' /\ s ≺ s')
-                                      \/ (exists t', u = s∙t' /\ t ≺ t').
-  Proof. 
-    inversion 1.
-    + left; exists s', t'; auto.
-    + right; exists t'; auto.
- Qed.
+    Hint Constructors bt_lt.
 
-  Fact bt_lt_irrefl s : ~ s ≺ s.
-  Proof.
-    intros H.
-    assert (forall t, s ≺ t -> s <> t) as D; [ | apply D in H; destruct H; auto ].
-    clear H; induction 1 as [ s t | s s' t H IH | s t t' H IH ]; try discriminate.
-    all: contradict IH; inversion IH; auto.
-  Qed.
+    Fact bt_lt_inv s t : s ≺ t -> s = ∅ /\ (exists u v, t = u⪧v)
+                               \/ (exists u u' v v', s = u⪧v /\ t = u'⪧v' /\ u ≺ u')
+                               \/ (exists u v v', s = u⪧v /\ t = u⪧v' /\ v ≺ v').
+    Proof.
+      destruct 1.
+      + left; split; auto; exists s, t; auto.
+      + right; left; exists s, s', t, t'; auto.
+      + do 2 right; exists s, t, t'; auto.
+    Qed.
 
-  Fact bt_lt_trans r s t : r ≺ s -> s ≺ t -> r ≺ t.
-  Proof.
-    intros H1; revert H1 t.
-    induction 1 as [ s t | s s' t t' H IH | s t t' H IH ]; intros u.
-    + inversion 1; auto.
-    + intros H1; apply bt_lt_node_inv in H1.
-      destruct H1 as [ (v & w & -> & ?) | (v & -> & ?) ];
-        constructor; auto.
-    + intros H1; apply bt_lt_node_inv in H1.
-      destruct H1 as [ (v & w & -> & ?) | (v & -> & ?) ].
-      * constructor; auto.
-      * constructor 3; auto.
-  Qed.
+    Fact bt_lt_node_inv s t u : s⪧t ≺ u -> (exists s' t', u = s'⪧t' /\ s ≺ s')
+                                        \/ (exists t', u = s⪧t' /\ t ≺ t').
+    Proof. 
+      inversion 1.
+      + left; exists s', t'; auto.
+      + right; exists t'; auto.
+    Qed.
+
+    Fact bt_lt_irrefl s : ~ s ≺ s.
+    Proof.
+      intros H.
+      assert (forall t, s ≺ t -> s <> t) as D; [ | apply D in H; destruct H; auto ].
+      clear H; induction 1 as [ s t | s s' t H IH | s t t' H IH ]; try discriminate.
+      all: contradict IH; inversion IH; auto.
+    Qed.
+
+    Fact bt_lt_trans r s t : r ≺ s -> s ≺ t -> r ≺ t.
+    Proof.
+      intros H1; revert H1 t.
+      induction 1 as [ s t | s s' t t' H IH | s t t' H IH ]; intros u.
+      + inversion 1; auto.
+      + intros H1; apply bt_lt_node_inv in H1.
+        destruct H1 as [ (v & w & -> & ?) | (v & -> & ?) ];
+          constructor; auto.
+      + intros H1; apply bt_lt_node_inv in H1.
+        destruct H1 as [ (v & w & -> & ?) | (v & -> & ?) ].
+        * constructor; auto.
+        * constructor 3; auto.
+    Qed.
   
-  Fact bt_lt_eq_lt_dec s t : { s ≺ t } + { s = t } + { t ≺ s }.
-  Proof.
-    revert t; induction s as [ | s1 H1 s2 H2 ]; intros [ | t1 t2 ]; auto.
-    destruct (H1 t1) as [ [ H3 | H3 ] | H3 ]; auto.
-    subst; destruct (H2 t2) as [ [] | ]; subst; auto.
-  Qed.
+    Fact bt_lt_eq_lt_dec s t : { s ≺ t } + { s = t } + { t ≺ s }.
+    Proof.
+      revert t; induction s as [ | s1 H1 s2 H2 ] using bt_rect; intros [ | t1 t2 ]; auto.
+      destruct (H1 t1) as [ [ H3 | H3 ] | H3 ]; auto.
+      subst; destruct (H2 t2) as [ [] | ]; subst; auto.
+    Qed.
 
-  Reserved Notation "x †" (at level 1).
-  Reserved Notation "x → y" (at level 3, right associativity).
+    Reserved Notation "x †" (at level 1).
+    Reserved Notation "x → y" (at level 3, right associativity).
 
-  Fixpoint bt_insert s t : bt :=
-    match t with
-      | ε   => s∙ε
-      | t∙u => match bt_lt_eq_lt_dec s t with
-        | inleft (left _)  => s∙t∙u
-        | inleft (right _) => t∙u
-        | inright _        => t∙(s→u)
+    Fixpoint bt_insert s t : bt :=
+      match t with
+        | ∅   => s⪧∅
+        | t⪧u => match bt_lt_eq_lt_dec s t with
+          | inleft (left _)  => s⪧t⪧u
+          | inleft (right _) => t⪧u
+          | inright _        => t⪧(s→u)
+        end
       end
-    end
-  where "s → t" := (bt_insert s t).
+    where "s → t" := (bt_insert s t).
 
-  Fact bt_lt_eq_lt_dec_refl s : exists H, bt_lt_eq_lt_dec s s = inleft (right H).
-  Proof.
-    destruct (bt_lt_eq_lt_dec s s) as [ [ C | H ] | C ].
-    1,3: exfalso; revert C; apply bt_lt_irrefl.
-    exists H; auto.
-  Qed.
+    Fact bt_lt_eq_lt_dec_refl s : exists H, bt_lt_eq_lt_dec s s = inleft (right H).
+    Proof.
+      destruct (bt_lt_eq_lt_dec s s) as [ [ C | H ] | C ].
+      1,3: exfalso; revert C; apply bt_lt_irrefl.
+      exists H; auto.
+    Qed.
 
-  Ltac bt_lt_eq H := match goal with |- context [bt_lt_eq_lt_dec ?x ?x] 
-         => destruct (bt_lt_eq_lt_dec_refl x) as (H & ->)
-    end.
+    Ltac bt_lt_eq H := 
+      match goal with 
+        |- context [bt_lt_eq_lt_dec ?x ?x] 
+             => destruct (bt_lt_eq_lt_dec_refl x) as (H & ->)
+      end.
 
-  Fact bt_insert_leaf s : s→ε = s∙ε.
-  Proof. reflexivity. Qed.
+    Fact bt_insert_leaf s : s→∅ = s⪧∅.
+    Proof. reflexivity. Qed.
 
-  Fact bt_insert_eq s t : s→s∙t = s∙t.
-  Proof.
-    simpl; bt_lt_eq H; auto.
-  Qed.
+    Fact bt_insert_eq s t : s→s⪧t = s⪧t.
+    Proof. simpl; bt_lt_eq H; auto. Qed.
 
-  Fact bt_insert_lt s t u : s ≺ t -> s→t∙u = s∙t∙u.
-  Proof.
-    intros H; simpl.
-    destruct (bt_lt_eq_lt_dec s t) as [ [C|C] | C ]; auto.
-    + contradict H; subst; apply bt_lt_irrefl.
-    + destruct (@bt_lt_irrefl s); apply bt_lt_trans with t; auto.
-  Qed.
+    Fact bt_insert_lt s t u : s ≺ t -> s→t⪧u = s⪧t⪧u.
+    Proof.
+      intros H; simpl.
+      destruct (bt_lt_eq_lt_dec s t) as [ [C|C] | C ]; auto.
+      + contradict H; subst; apply bt_lt_irrefl.
+      + destruct (@bt_lt_irrefl s); apply bt_lt_trans with t; auto.
+    Qed.
 
-  Fact bt_insert_gt s t u : t ≺ s -> s→t∙u = t∙(s→u).
-  Proof.
-    intros H; simpl.
-    destruct (bt_lt_eq_lt_dec s t) as [ [C|C] | C ]; auto.
-    + destruct (@bt_lt_irrefl s); apply bt_lt_trans with t; auto.
-    + contradict H; subst; apply bt_lt_irrefl.
-  Qed.
+    Fact bt_insert_gt s t u : t ≺ s -> s→t⪧u = t⪧(s→u).
+    Proof.
+      intros H; simpl.
+      destruct (bt_lt_eq_lt_dec s t) as [ [C|C] | C ]; auto.
+      + destruct (@bt_lt_irrefl s); apply bt_lt_trans with t; auto.
+      + contradict H; subst; apply bt_lt_irrefl.
+    Qed.
 
-  Fact bt_insert_equiv s t : s→t ≈ s∙t.
-  Proof.
-    induction t as [ | t Ht u Hu ]; simpl; auto.
-    destruct (bt_lt_eq_lt_dec s t) as [ [] | ]; subst; auto.
-    apply bte_trans with (t∙s∙u); auto.
-  Qed.
+    Fact bt_insert_equiv s t : s→t ≈ s⪧t.
+    Proof.
+      induction t as [ | t u Hu ] using bt_rect'; simpl; auto.
+      destruct (bt_lt_eq_lt_dec s t) as [ [] | ]; subst; auto.
+      apply bte_trans with (t⪧s⪧u); auto.
+    Qed.
 
-  Fixpoint bt_norm t :=
-    match t with
-      | ε   => ε
-      | s∙t => s† → t†
-    end
-  where "t †" := (bt_norm t).
+    Fixpoint bt_norm t :=
+      match t with
+        | ∅   => ∅
+        | s⪧t => s† → t†
+      end
+    where "t †" := (bt_norm t).
 
-  Hint Resolve bt_insert_equiv.
+    Hint Resolve bt_insert_equiv.
   
-  Fact bt_norm_eq t : t† ≈ t.
-  Proof.
-    induction t as [ | s ? t ? ]; simpl; auto.
-    apply bte_trans with (s†∙t†); auto.
-  Qed.
+    Fact bt_norm_eq t : t† ≈ t.
+    Proof.
+      induction t as [ | s ? t ? ]; simpl; auto.
+      apply bte_trans with (s†⪧t†); auto.
+    Qed.
 
-  Opaque bt_insert.
+    Opaque bt_insert.
 
-  Tactic Notation "rew" "bt" "insert" := 
-    repeat match goal with 
-      |             |- context[_→ε]     => rewrite bt_insert_leaf
-      |             |- context[?x→?x∙_] => rewrite bt_insert_eq
-      | H : ?x ≺ ?y |- context[?x→?y∙_] => rewrite bt_insert_lt with (1 := H)
-      | H : ?x ≺ ?y |- context[?y→?x∙_] => rewrite bt_insert_gt with (1 := H)
-    end.
+    Tactic Notation "rew" "bt" "insert" := 
+      repeat match goal with 
+        |             |- context[_→∅]     => rewrite bt_insert_leaf
+        |             |- context[?x→?x⪧_] => rewrite bt_insert_eq
+        | H : ?x ≺ ?y |- context[?x→?y⪧_] => rewrite bt_insert_lt with (1 := H)
+        | H : ?x ≺ ?y |- context[?y→?x⪧_] => rewrite bt_insert_gt with (1 := H)
+      end.
 
-  Tactic Notation "bt" "insert" "case" hyp(x) hyp(y) :=
-    destruct (bt_lt_eq_lt_dec x y) as [ [|] | ]; subst; rew bt insert; auto.
+    Tactic Notation "bt" "insert" "case" hyp(x) hyp(y) :=
+      destruct (bt_lt_eq_lt_dec x y) as [ [|] | ]; subst; rew bt insert; auto.
 
-  Tactic Notation "bt" "lt" "trans" constr(t) := apply bt_lt_trans with t; auto.
+    Tactic Notation "bt" "lt" "trans" constr(t) := apply bt_lt_trans with t; auto.
 
-  Tactic Notation "bt" "lt" "cycle" :=
-    match goal with
-      | H1 : ?x ≺ ?x |- _  => destruct (@bt_lt_irrefl x); auto
-      | H1 : ?x ≺ ?y, 
-        H2 : ?y ≺ ?x |- _  => destruct (@bt_lt_irrefl x); bt lt trans y
-      | H1 : ?x ≺ ?y,
-        H2 : ?y ≺ ?z,
-        H3 : ?z ≺ ?x |- _  => destruct (@bt_lt_irrefl x); bt lt trans y; bt lt trans z
-    end.
+    Tactic Notation "bt" "lt" "cycle" :=
+      match goal with
+        | H1 : ?x ≺ ?x |- _  => destruct (@bt_lt_irrefl x); auto
+        | H1 : ?x ≺ ?y, 
+          H2 : ?y ≺ ?x |- _  => destruct (@bt_lt_irrefl x); bt lt trans y
+        | H1 : ?x ≺ ?y,
+          H2 : ?y ≺ ?z,
+          H3 : ?z ≺ ?x |- _  => destruct (@bt_lt_irrefl x); bt lt trans y; bt lt trans z
+      end.
 
-  Fact bt_insert_cntr s t : s→s→t = s→t.
-  Proof.
-    induction t as [ | t1 IH1 t2 IH2 ]; rew bt insert; auto.
-    bt insert case s t1; f_equal; auto.
-  Qed.
+    Fact bt_insert_cntr s t : s→s→t = s→t.
+    Proof.
+      induction t as [ | t1 t2 IH2 ] using bt_rect'; rew bt insert; auto.
+      bt insert case s t1; f_equal; auto.
+    Qed.
 
-  Fact bt_insert_comm s t u : s→t→u = t→s→u.
-  Proof.
-    induction u as [ | u1 IH1 u2 IH2 ]. 
-    + rew bt insert; bt insert case s t.
-    + bt insert case t u1; 
-      bt insert case s u1; 
-      bt insert case s t; 
-      try bt lt cycle; 
-      f_equal; auto.
-  Qed.
+    Fact bt_insert_comm s t u : s→t→u = t→s→u.
+    Proof.
+      induction u as [ | u1 u2 IH ] using bt_rect'. 
+      + rew bt insert; bt insert case s t.
+      + bt insert case t u1; 
+        bt insert case s u1; 
+        bt insert case s t; 
+        try bt lt cycle; 
+        f_equal; auto.
+    Qed.
 
-  Hint Resolve bt_insert_cntr bt_insert_comm bt_norm_eq.
+    Hint Resolve bt_insert_cntr bt_insert_comm bt_norm_eq.
 
-  Theorem bte_norm_iff s t : s ≈ t <-> s† = t†.
-  Proof.
-    split.
-    + induction 1; simpl; auto.
-      * transitivity s†; auto.
-      * f_equal; auto.
-    + intros H.
-      apply bte_trans with s †; auto.
-      rewrite H; auto.
-  Qed.
+    Theorem bte_norm_iff s t : s ≈ t <-> s† = t†.
+    Proof.
+      split.
+      + induction 1; simpl; auto.
+        * transitivity s†; auto.
+        * f_equal; auto.
+      + intros H.
+        apply bte_trans with s †; auto.
+        rewrite H; auto.
+    Qed.
 
-  Theorem bt_norm_idem s : s†† = s†.
-  Proof. apply bte_norm_iff; auto. Qed.
+    Theorem bt_norm_idem s : s†† = s†.
+    Proof. apply bte_norm_iff; auto. Qed.
 
-  Fact bte_dec s t : { s ≈ t } + { s ≉ t }.
-  Proof.
-    destruct (bt_eq_dec s† t†) as [ H | H ];
-    rewrite <- bte_norm_iff in H; auto.
-  Qed.
+    Theorem bte_dec s t : { s ≈ t } + { s ≉ t }.
+    Proof.
+      destruct (bt_eq_dec s† t†) as [ H | H ];
+      rewrite <- bte_norm_iff in H; auto.
+    Qed.
 
-  Corollary btm_dec s t : { s ∊ t } + { ~ s ∊ t }.
+  End establishing_decidability.
+
+  Corollary btm_dec s t : { s ∈ t } + { ~ s ∈ t }.
   Proof. apply bte_dec. Qed.
 
-  Opaque max.
+  Section more_decidability.
 
-  Fact bte_depth_eq s t : s ≈ t -> ⌞s⌟ = ⌞t⌟.
-  Proof.
-    induction 1; simpl; auto.
-    + transitivity ⌞s⌟; auto.
-    + rewrite max_assoc, max_idempotent; auto.
-    + rewrite max_assoc, (max_comm (S _)), max_assoc; auto.
-  Qed.
+    Section btm_ex_dec.
+  
+      Variable (P : bt -> Prop) (HP : forall s t, s ≈ t -> P s -> P t).
 
-  Fact btm_depth s t : s ∊ t -> ⌞s⌟ < ⌞t⌟.
-  Proof.
-    intros H; apply bte_depth_eq in H; simpl in H.
-    rewrite <- H.
-    apply lt_le_trans with (1 := lt_n_Sn _).
-    apply le_max_l.
-  Qed.
+      Theorem btm_ex_dec t : (forall x, x ∈ t -> { P x } + { ~ P x })
+                       -> { s | s ∈ t /\ P s } + { forall s, s ∈ t -> ~ P s }.
+      Proof.
+        induction t as [ | s t IHt ] using bt_rect'; intros Ht.
+        + right; intros ?; rewrite btm_inv_0; tauto.
+        + destruct (Ht s) as [ H | H ]; auto.
+          * left; exists s; auto.
+          * destruct IHt as [ (x & H1 & H2) | H1 ].
+            - intros x Hx; apply Ht, btm_inv; auto.
+            - left; exists x; rewrite btm_inv; auto.
+            - right; intros x; rewrite btm_inv.
+              intros [ | ]; auto.
+              contradict H; revert H; apply HP; auto.
+      Qed.
 
-  (** bt is well-founded for membership *)
+    End btm_ex_dec.
 
-  Theorem btm_wf : well_founded (fun s t => s ∊ t).
-  Proof.
-    apply wf_incl with (1 := btm_depth).
-    apply wf_inverse_image, lt_wf.
-  Qed.
+    Corollary btm_fa_dec (P : _ -> Prop) t : 
+                             (forall s t, s ≈ t -> P s -> P t)
+                          -> (forall x, x ∈ t -> { P x } + { ~ P x })
+                          -> { s | s ∈ t /\ ~ P s } + { forall s, s ∈ t -> P s }.
+    Proof.
+      intros H1 H2.
+      destruct btm_ex_dec with (P := fun x => ~ P x) (t := t)
+        as [ H | H ]; auto.
+      + intros u v G1 G2; contradict G2; revert G2; apply H1; auto.
+      + intros x Hx; specialize (H2 _ Hx); tauto.
+      + right; intros s Hs; specialize (H _ Hs).
+        destruct (H2 _ Hs); tauto.
+    Qed.
 
-  Notation "∊-chain" := (chain (fun s t => s ∊ t)).
+    Definition btm_select (P : _ -> Prop) t :
+                             (forall s t, s ≈ t -> P s -> P t)
+                          -> (forall x, x ∈ t -> { P x } + { ~ P x })
+                          -> { s | forall x, x ∈ s <-> x ∈ t /\ P x }.
+    Proof.
+      intros HP0.
+      induction t as [ | s t Ht ] using bt_rect'; intros HP.
+      + exists ∅; intros s; rewrite btm_inv_0; tauto.
+      + destruct Ht as (t' & H').
+        * intros x Hx; apply HP, btm_inv; auto.
+        * destruct (HP s) as [ H | H ]; auto.
+          - exists (s⪧t'); intros x; rewrite btm_inv, btm_inv, H'.
+            split; try tauto.
+            intros [ H1 | (H1 & H2) ]; auto.
+            split; auto.
+            revert H; apply HP0; auto.
+          - exists t'; intros x; rewrite btm_inv, H'.
+            split; try tauto.
+            intros ([H1|H1] & H2); split; auto.
+            contradict H; revert H2; apply HP0; auto.
+    Qed.
+  
+    Definition btm_partition x s : x ∈ s -> { t | s ≈ x⪧t /\ ~ x ∈ t }.
+    Proof.
+      induction s as [ | y s IHs ] using bt_rect'.
+      + intros H; exfalso; revert H; rewrite btm_inv_0; intros [].
+      + intros H; rewrite btm_inv in H.
+        destruct (bte_dec x y) as [ H1 | H1 ]; 
+        destruct (btm_dec x s) as [ H2 | H2 ]; try (exfalso; tauto). 
+        * destruct (IHs H2) as (t & H3 & H4).
+          exists t; split; auto.
+          apply bte_trans with (y⪧x⪧t); auto.
+          apply btm_inv; auto.
+        * exists s; auto.
+        * destruct (IHs H2) as (t & H3 & H4).
+          exists (y⪧t); split; auto.
+          - apply bte_trans with (y⪧x⪧t); auto.
+          - contradict H4.
+            apply btm_inv in H4; tauto.
+    Qed.
 
-  Fact btm_chain_depth n s t : ∊-chain n s t -> n+⌞s⌟ <= ⌞t⌟.
-  Proof.
-    induction 1 as [ | n s t u H1 H2 IH2 ]; auto.
-    apply le_trans with (2 := IH2).
-    apply btm_depth in H1; lia.
-  Qed.
+  End more_decidability.
 
-  Fact btm_chain_congr_r n s t t' : t ≈ t' -> ∊-chain (S n)  s t -> ∊-chain (S n) s t'.
-  Proof.
-    intros H1 H2.
-    apply chain_snoc_inv in H2.
-    destruct H2 as (y & H2 & H3).
-    apply chain_snoc with y; auto.
-    revert H3; apply btm_congr_r; auto.
-  Qed.
+  Notation "∈-chain" := (chain (fun s t => s ∈ t)).
+  Notation "∈-chain_list" := (chain_list (fun s t => s ∈ t)).
 
-  Notation "∊-chain_list" := (chain_list (fun s t => s ∊ t)).
- 
-  Fact btm_chain_list_comp u l s t : l <> nil
-                              -> ∊-chain_list l s t
-                              -> ∊-chain_list l s (u∙t).
-  Proof.
-    rewrite <- (rev_involutive l).
-    generalize (rev l); clear l; intros l Hl.
-    destruct l as [ | x l ].
-    { destruct Hl; auto. }
-    clear Hl.
-    simpl; intros H.
-    apply chain_list_app_inv in H.
-    destruct H as (v & H1 & H2).
-    apply chain_list_app with v; auto.
-    apply chain_list_cons_inv in H2.
-    destruct H2 as (-> & k & H2 & H3).
-    apply chain_list_nil_inv in H3; subst k.
-    constructor 2 with (u∙t); auto.
-    + apply btm_inv; auto.
-    + constructor.
-  Qed.
+  Section bte_depth_and_chains.
 
-  Fact btm_chain_comp n u s t : ∊-chain (S n) s t -> ∊-chain (S n) s (u∙t).
-  Proof.
-    intros H.
-    apply chain_chain_list in H.
-    destruct H as (l & H1 & H2).
-    rewrite H2. 
-    apply chain_list_chain.
-    apply btm_chain_list_comp; auto.
-    destruct l; discriminate.
-  Qed.
+    Opaque max.
 
-  Fact btm_depth_chain t : { l | ∊-chain_list l ε t /\ length l = ⌞t⌟ }.
-  Proof.
-    induction t as [ | s (ls & H1 & H2) t (lt & H3 & H4) ].
-    + exists nil; simpl; split; auto; constructor.
-    + destruct (le_lt_dec (S ⌞s⌟) ⌞t⌟) as [ H | H ].
-      * exists lt; simpl; split.
-        - apply btm_chain_list_comp; auto.
-          destruct lt; try discriminate; simpl in *; lia.
-        - rewrite max_r; auto.
-      * exists (ls++s::nil); split.
-        - apply chain_list_app with (1 := H1).
-          constructor 2 with (s∙t); auto.
-          constructor.
-        - rewrite app_length; simpl.
-          rewrite max_l; lia.
-  Qed.
+    Fact bte_depth_eq s t : s ≈ t -> ⌞s⌟ = ⌞t⌟.
+    Proof.
+      induction 1; simpl; auto.
+      + transitivity ⌞s⌟; auto.
+      + rewrite max_assoc, max_idempotent; auto.
+      + rewrite max_assoc, (max_comm (S _)), max_assoc; auto.
+    Qed.
 
-  Fact bt_chain_inv_0 n x : ∊-chain n x ε -> n = 0 /\ x = ε.
-  Proof.
-    assert (forall y, ∊-chain n x y -> y = ε -> n = 0 /\ x = ε) as H.
-    { induction 1 as [ | n x y z H1 H2 IH2 ]; auto.
-      intros ->; destruct IH2 as (_ & ->); auto.
-      apply bte_discr in H1; tauto. }
-    intros G; apply (H _ G); auto.
-  Qed.
+    Fact btm_depth s t : s ∈ t -> ⌞s⌟ < ⌞t⌟.
+    Proof.
+      intros H; apply bte_depth_eq in H; simpl in H.
+      rewrite <- H.
+      apply lt_le_trans with (1 := lt_n_Sn _).
+      apply le_max_l.
+    Qed.
 
-  (* Up to ≈, membership in t is finite *)
+    (** bt is well-founded for membership *)
 
-  Theorem btm_finite_t t : { l | forall s, s ∊ t <-> exists s', s ≈ s' /\ In s' l }.
+    Theorem btm_wf : well_founded (fun s t => s ∈ t).
+    Proof.
+      apply wf_incl with (1 := btm_depth),
+            wf_inverse_image, lt_wf.
+    Qed.
+
+    Fact btm_chain_depth n s t : ∈-chain n s t -> n+⌞s⌟ <= ⌞t⌟.
+    Proof.
+      induction 1 as [ | n s t u H1 H2 IH2 ]; auto.
+      apply le_trans with (2 := IH2).
+      apply btm_depth in H1; lia.
+    Qed.
+
+    Fact btm_chain_congr_r n s t t' : t ≈ t' -> ∈-chain (S n)  s t -> ∈-chain (S n) s t'.
+    Proof.
+      intros H1 H2.
+      apply chain_snoc_inv in H2.
+      destruct H2 as (y & H2 & H3).
+      apply chain_snoc with y; auto.
+      revert H3; apply btm_congr_r; auto.
+    Qed.
+
+    Fact btm_chain_list_comp u l s t : l <> nil
+                              -> ∈-chain_list l s t
+                              -> ∈-chain_list l s (u⪧t).
+    Proof.
+      rewrite <- (rev_involutive l).
+      generalize (rev l); clear l; intros l Hl.
+      destruct l as [ | x l ].
+      { destruct Hl; auto. }
+      clear Hl.
+      simpl; intros H.
+      apply chain_list_app_inv in H.
+      destruct H as (v & H1 & H2).
+      apply chain_list_app with v; auto.
+      apply chain_list_cons_inv in H2.
+      destruct H2 as (-> & k & H2 & H3).
+      apply chain_list_nil_inv in H3; subst k.
+      constructor 2 with (u⪧t); auto.
+      + apply btm_inv; auto.
+      + constructor.
+    Qed.
+
+    Fact btm_chain_comp n u s t : ∈-chain (S n) s t -> ∈-chain (S n) s (u⪧t).
+    Proof.
+      intros H.
+      apply chain_chain_list in H.
+      destruct H as (l & H1 & H2).
+      rewrite H2. 
+      apply chain_list_chain.
+      apply btm_chain_list_comp; auto.
+      destruct l; discriminate.
+    Qed.
+
+    Fact btm_depth_chain t : { l | ∈-chain_list l ∅ t /\ length l = ⌞t⌟ }.
+    Proof.
+      induction t as [ | s (ls & H1 & H2) t (lt & H3 & H4) ].
+      + exists nil; simpl; split; auto; constructor.
+      + destruct (le_lt_dec (S ⌞s⌟) ⌞t⌟) as [ H | H ].
+        * exists lt; simpl; split.
+          - apply btm_chain_list_comp; auto.
+            destruct lt; try discriminate; simpl in *; lia.
+          - rewrite max_r; auto.
+        * exists (ls++s::nil); split.
+          - apply chain_list_app with (1 := H1).
+            constructor 2 with (s⪧t); auto.
+            constructor.
+          - rewrite app_length; simpl.
+            rewrite max_l; lia.
+    Qed.
+
+    Fact bt_chain_inv_0 n x : ∈-chain n x ∅ -> n = 0 /\ x = ∅.
+    Proof.
+      assert (forall y, ∈-chain n x y -> y = ∅ -> n = 0 /\ x = ∅) as H.
+      { induction 1 as [ | n x y z H1 H2 IH2 ]; auto.
+        intros ->; destruct IH2 as (_ & ->); auto.
+        apply bte_discr in H1; tauto. }
+      intros G; apply (H _ G); auto.
+    Qed.
+
+  End bte_depth_and_chains.
+
+  (** Very important to build the finite HF-model 
+
+      Up to ≈, membership in t is finite *)
+
+  Theorem btm_finite_t t : { l | forall s, s ∈ t <-> exists s', s ≈ s' /\ In s' l }.
   Proof.
     induction t as [ | s (ls & Hs) t (lt & Ht) ].
     + exists nil; intros s.
@@ -487,89 +615,9 @@ Section btree.
         right; exists s'; auto.
   Qed.
 
-  Reserved Notation "x ∪ y" (at level 60, right associativity).
+  Notation "x ⊆ y" := (forall u, u ∈ x -> u ∈ y) (at level 70).
 
-  Fixpoint bt_cup s t := 
-    match s with 
-      | ε   => t
-      | x∙s => x∙(s ∪ t)
-    end
-  where "s ∪ t" := (bt_cup s t).
-
-  Theorem bt_cup_spec x s t : x ∊ s ∪ t <-> x ∊ s \/ x ∊ t.
-  Proof.
-    revert x; induction s as [ | y Hy s Hs ]; intros x; simpl.
-    + rewrite btm_inv_0; tauto.
-    + rewrite btm_inv, btm_inv, Hs; tauto.
-  Qed.
-
-  Reserved Notation "↓ x" (at level 1).
-
-  Fixpoint bt_ct t := 
-    match t with 
-      | ε   => ε
-      | s∙t => s∙(↓s ∪ ↓t)
-    end
-  where "↓ t" := (bt_ct t).
-
-  Fact bt_ct_congr_l u v t : u ≈ v -> u ∊ ↓t -> v ∊ ↓t.
-  Proof.
-    revert u v; induction t; simpl; intros ? ? ?; apply btm_congr_l; auto.
-  Qed.
-
-  Fact bt_ct_congr_r u s t : s ≈ t -> u ∊ ↓s <-> u ∊ ↓t.
-  Proof.
-    intros H; revert H u. 
-    induction 1 as [ | s t | r s t H1 IH1 H2 IH2 | s t | s t u 
-                   | s s' t t' H1 IH1 H2 IH2 ]; intros v; try tauto.
-    + symmetry; auto.
-    + rewrite IH1; auto.
-    + simpl; repeat (rewrite btm_inv || rewrite bt_cup_spec); tauto.
-    + simpl; repeat (rewrite btm_inv || rewrite bt_cup_spec); tauto.
-    + simpl; repeat (rewrite btm_inv || rewrite bt_cup_spec).
-      rewrite IH1, IH2; split; intros [ H | [] ]; auto; left.
-      * apply bte_trans with s; auto.
-      * apply bte_trans with s'; auto.
-  Qed.
-
-  (** The transitive closure is composed of the x st x ∊ ... ∊ t *)
-
-  Theorem bt_ct_spec t x : x ∊ ↓t <-> exists n, ∊-chain (S n) x t.
-  Proof.
-    revert x; induction t as [ | s Hs t Ht ]; intros x; simpl.
-    + rewrite btm_inv_0; split; try tauto.
-      intros (n & Hn).
-      apply chain_inv_S in Hn.
-      destruct Hn as (y & H1 & H2).
-      apply bt_chain_inv_0 in H2.
-      destruct H2 as (_ & ->).
-      apply bte_discr in H1; tauto.
-    + rewrite btm_inv, bt_cup_spec, Hs, Ht.
-      split.
-      * intros [ H | [ (n & H) | (n & H) ] ].
-        - exists 0.
-          constructor 2 with (s∙t).
-          ++ apply btm_inv; auto.
-          ++ constructor.
-        - exists (S n).
-          apply chain_snoc with s; auto.
-        - exists n; apply btm_chain_comp; auto.
-      * intros (n & H).
-        apply chain_snoc_inv in H.
-        destruct H as (y & H1 & H2).
-        apply btm_inv in H2.
-        destruct H2 as [ H2 | H2 ].
-        - destruct n as [ | n ].
-          ++ apply chain_inv_0 in H1; subst; auto.
-          ++ right; left; exists n.
-             revert H1; apply btm_chain_congr_r; auto.
-        - right; right; exists n.
-          apply chain_snoc with y; auto.
-  Qed.
-
-  Notation "x ⊆ y" := (forall u, u ∊ x -> u ∊ y) (at level 70).
-
-  Fact bti_inv_0 x : x ⊆ ε <-> x = ε.
+  Fact bti_inv_0 x : x ⊆ ∅ <-> x = ∅.
   Proof.
     split; intros H; subst; auto.
     destruct x as [ | s t ]; auto.
@@ -578,94 +626,18 @@ Section btree.
     destruct H; auto.
   Qed.
 
-  Section btm_dec.
-
-    Variable (P : bt -> Prop) (HP : forall s t, s ≈ t -> P s -> P t).
-
-    Theorem btm_ex_dec t : (forall x, x ∊ t -> { P x } + { ~ P x })
-                     -> { s | s ∊ t /\ P s } + { forall s, s ∊ t -> ~ P s }.
-    Proof.
-      induction t as [ | s _ t IHt ]; intros Ht.
-      + right; intros ?; rewrite btm_inv_0; tauto.
-      + destruct (Ht s) as [ H | H ]; auto.
-        * left; exists s; auto.
-        * destruct IHt as [ (x & H1 & H2) | H1 ].
-          - intros x Hx; apply Ht, btm_inv; auto.
-          - left; exists x; rewrite btm_inv; auto.
-          - right; intros x; rewrite btm_inv.
-            intros [ | ]; auto.
-            contradict H; revert H; apply HP; auto.
-    Qed.
-
-  End btm_dec.
-
-  Corollary btm_fa_dec (P : _ -> Prop) t : 
-                             (forall s t, s ≈ t -> P s -> P t)
-                          -> (forall x, x ∊ t -> { P x } + { ~ P x })
-                          -> { s | s ∊ t /\ ~ P s } + { forall s, s ∊ t -> P s }.
-  Proof.
-    intros H1 H2.
-    destruct btm_ex_dec with (P := fun x => ~ P x) (t := t)
-      as [ H | H ]; auto.
-    + intros u v G1 G2; contradict G2; revert G2; apply H1; auto.
-    + intros x Hx; specialize (H2 _ Hx); tauto.
-    + right; intros s Hs; specialize (H _ Hs).
-      destruct (H2 _ Hs); tauto.
-  Qed.
-
-  Definition btm_select (P : _ -> Prop) t :
-                             (forall s t, s ≈ t -> P s -> P t)
-                          -> (forall x, x ∊ t -> { P x } + { ~ P x })
-                          -> { s | forall x, x ∊ s <-> x ∊ t /\ P x }.
-  Proof.
-    intros HP0.
-    induction t as [ | s _ t Ht ]; intros HP.
-    + exists ε; intros s; rewrite btm_inv_0; tauto.
-    + destruct Ht as (t' & H').
-      * intros x Hx; apply HP, btm_inv; auto.
-      * destruct (HP s) as [ H | H ]; auto.
-        - exists (s∙t'); intros x; rewrite btm_inv, btm_inv, H'.
-          split; try tauto.
-          intros [ H1 | (H1 & H2) ]; auto.
-          split; auto.
-          revert H; apply HP0; auto.
-        - exists t'; intros x; rewrite btm_inv, H'.
-          split; try tauto.
-          intros ([H1|H1] & H2); split; auto.
-          contradict H; revert H2; apply HP0; auto.
-  Qed.
-  
-  Definition btm_partition x s : x ∊ s -> { t | s ≈ x∙t /\ ~ x ∊ t }.
-  Proof.
-    induction s as [ | y _ s IHs ].
-    + intros H; exfalso; revert H; rewrite btm_inv_0; intros [].
-    + intros H; rewrite btm_inv in H.
-      destruct (bte_dec x y) as [ H1 | H1 ]; 
-      destruct (btm_dec x s) as [ H2 | H2 ]; try (exfalso; tauto). 
-      * destruct (IHs H2) as (t & H3 & H4).
-        exists t; split; auto.
-        apply bte_trans with (y∙x∙t); auto.
-        apply btm_inv; auto.
-      * exists s; auto.
-      * destruct (IHs H2) as (t & H3 & H4).
-        exists (y∙t); split; auto.
-        - apply bte_trans with (y∙x∙t); auto.
-        - contradict H4.
-          apply btm_inv in H4; tauto.
-  Qed.
-
   Fact bti_refl x : x ⊆ x.
   Proof. auto. Qed.
 
   Fact bti_trans x y z : x ⊆ y -> y ⊆ z -> x ⊆ z.
   Proof. intros H1 H2 k Hx; apply H2, H1; auto. Qed.
 
-  Fact bti_comp s t : t ⊆ s∙t.
+  Fact bti_comp s t : t ⊆ s⪧t.
   Proof.
     intros x; rewrite btm_inv; auto.
   Qed.
 
-  Fact bti_mono_r x s t : s ⊆ t -> x∙s ⊆ x∙t.
+  Fact bti_mono_r x s t : s ⊆ t -> x⪧s ⊆ x⪧t.
   Proof.
     intros H z; do 2 rewrite btm_inv; intros []; auto.
   Qed.
@@ -675,7 +647,7 @@ Section btree.
     intros H x; apply btm_congr_r; auto.
   Qed.
 
-  Fact btm_bti x s : x ∊ s -> x∙s ⊆ s.
+  Fact btm_bti x s : x ∈ s -> x⪧s ⊆ s.
   Proof. intro; apply bte_bti; auto. Qed.
 
   Fact bti_congr_l x y t : x ≈ y -> x ⊆ t-> y ⊆ t.
@@ -694,7 +666,7 @@ Section btree.
 
   Fact bti_dec s t : { s ⊆ t } + { ~ s ⊆ t }.
   Proof.
-    destruct btm_fa_dec with (P := fun x => x ∊ t) (t := s)
+    destruct btm_fa_dec with (P := fun x => x ∈ t) (t := s)
       as [ (x & H1 & H2) | H1 ]; auto.
     + intros ? ?; apply btm_congr_l.
     + intros ? ?; apply btm_dec.
@@ -702,7 +674,7 @@ Section btree.
 
   Fact bti_equiv s t : s ⊆ t -> t ⊆ s -> s ≈ t.
   Proof.
-    revert t; induction s as [ | x _ s Hs ].
+    revert t; induction s as [ | x s Hs ] using bt_rect'.
     + intros t _ Ht.
       destruct t as [ | y t ]; auto.
       specialize (Ht y).
@@ -718,25 +690,35 @@ Section btree.
           apply Hs.
           ++ apply bti_trans with (2 := H1); auto.
           ++ apply bti_trans with (1 := H2), btm_bti; auto.
-        - assert (x ∊ y∙t) as H4 by (apply H1; auto).
+        - assert (x ∈ y⪧t) as H4 by (apply H1; auto).
           destruct btm_partition with (1 := H4)
             as (u & H5 & H6).
           assert (s ≈ u) as H7.
           { apply Hs.
             + intros z Hz.
-              assert (z ∊ x∙u) as H7.
+              assert (z ∈ x⪧u) as H7.
               { apply btm_congr_r with (1 := H5), H1, btm_inv; auto. }
               apply btm_inv in H7; destruct H7 as [ H7 | ]; auto.
               contradict H3; revert Hz; apply btm_congr_l; auto.
             + intros z Hz.
-              assert (z ∊ x∙s) as H7.
+              assert (z ∈ x⪧s) as H7.
               { apply H2, btm_congr_r with (1 := in_bte_sym H5), btm_inv; auto. }
               apply btm_inv in H7; destruct H7 as [ H7 | ]; auto.
               contradict H6; revert Hz; apply btm_congr_l; auto. }
-          apply bte_trans with (x∙u); auto.
+          apply bte_trans with (x⪧u); auto.
   Qed.
 
-  Fact bti_inv x s t : x ⊆ s∙t <-> x ⊆ t \/ exists y, y ⊆ t /\ x ≈ s∙y.
+  Fact bte_incl_equiv s t : s ≈ t <-> s ⊆ t /\ t ⊆ s.
+  Proof.
+    split.
+    + intros H; split; apply bte_bti; auto.
+    + intros []; apply bti_equiv; auto.
+  Qed.
+
+  Fact bte_ext s t : s ≈ t <-> forall x, x ∈ s <-> x ∈ t.
+  Proof. rewrite bte_incl_equiv; firstorder. Qed.
+
+  Fact bti_inv x s t : x ⊆ s⪧t <-> x ⊆ t \/ exists y, y ⊆ t /\ x ≈ s⪧y.
   Proof.
     split.
     + intros H.
@@ -745,7 +727,7 @@ Section btree.
           as (y & H2 & H3).
         right; exists y; split; auto.
         intros z Hz.
-        assert (z ∊ s∙t) as C.
+        assert (z ∈ s⪧t) as C.
         { apply H.
           apply btm_congr_r with (1 := in_bte_sym H2), btm_inv; auto. }
         apply btm_inv in C; destruct C as [C|]; auto.
@@ -762,146 +744,20 @@ Section btree.
       * intros z Hz.
         apply bti_congr_r with (1 := H2) in Hz; auto.
         revert Hz; do 2 rewrite btm_inv; intros []; auto.
-  Qed.   
-
-  Fact bt_ct_incr t : t ⊆ ↓t.
-  Proof.
-    intro; induction t; simpl; auto.
-    rewrite btm_inv, btm_inv, bt_cup_spec; tauto.
   Qed.
 
-  Fact bt_ct_mono s t : s ⊆ t -> ↓s ⊆ ↓t.
+  Fixpoint bt_cup s t := 
+    match s with 
+      | ∅   => t
+      | x⪧s => x⪧(s ∪ t)
+    end
+  where "s ∪ t" := (bt_cup s t).
+
+  Theorem bt_cup_spec x s t : x ∈ s ∪ t <-> x ∈ s \/ x ∈ t.
   Proof.
-    intros H x.
-    do 2 rewrite bt_ct_spec.
-    intros (n & Hn).
-    apply chain_snoc_inv in Hn.
-    destruct Hn as (y & H1 & H2).
-    exists n; apply chain_snoc with y; auto.
-  Qed.
-
-  Hint Resolve bt_ct_incr bt_ct_mono.
-
-  Definition bt_transitive t := forall u v, u ∊ v -> v ∊ t -> u ∊ t.
-
-  Theorem bt_ct_trans t : bt_transitive ↓t.
-  Proof.
-    induction t as [ | s Hs t Ht ]; simpl; intros u v H1 H2.
-    + apply btm_inv_0 in H2; tauto.
-    + apply btm_inv in H2.
-      rewrite bt_cup_spec in H2.
-      rewrite btm_inv, bt_cup_spec.
-      destruct H2 as [ H2 | [ H2 | H2 ] ].
-      * right; left; apply bt_ct_congr_r with (1 := H2); auto.
-      * right; left; revert H2; apply Hs; auto.
-      * right; right; revert H2; apply Ht; auto.
-  Qed.
-
-  Hint Resolve bt_ct_trans.
-
-  Fact bt_trans_chain n x y t : bt_transitive t -> ∊-chain n x y -> y ∊ t -> x ∊ t. 
-  Proof.
-    intros Ht; induction 1 as [ | n x y z H1 H2 IH2 ]; auto.
-    intros H; apply Ht with (1 := H1); auto.
-  Qed.
-
-  Fact bt_ct_idem t : ↓(↓t) ⊆ ↓t.
-  Proof.
-    intros x; rewrite bt_ct_spec.
-    intros (n & Hn).
-    apply chain_snoc_inv in Hn.
-    destruct Hn as (y & H1 & H2).
-    revert H1 H2.
-    apply bt_trans_chain; auto.
-  Qed.
-
-  Fixpoint bt_bcup x t :=
-    match t with
-      | ε   => ε 
-      | s∙t => (x∙s) ∪ (bt_bcup x t)
-    end.
-
-  Fact bt_bcup_spec x t u : u ∊ bt_bcup x t <-> exists k, u ∊ x∙k /\ k ∊ t.
-  Proof.
-    revert u; induction t as [ | s Hs t Ht ]; intros u; simpl.
-    + rewrite btm_inv_0; split; try tauto.
-      intros (k & _ & Hk); revert Hk; rewrite btm_inv_0; auto.
-    + rewrite btm_inv, bt_cup_spec; split.
-      * intros [ H | [ H | H ] ].
-        - exists s; split; auto.
-          apply btm_congr_l with x; auto.
-        - exists s; split; auto.
-        - rewrite Ht in H.
-          destruct H as (k & ? & ?).
-          exists k; split; auto.
-      * intros (k & H1 & H2); revert H1 H2.
-        rewrite btm_inv, btm_inv.
-        intros [H1|H1] [H2|H2]; auto.
-        - right; left; revert H1; apply btm_congr_r; auto.
-        - right; right; apply Ht; exists k.
-          rewrite btm_inv; auto.
-  Qed.
-
-  Fixpoint bt_mcomp x t :=
-    match t with
-      | ε   => ε 
-      | s∙t => (x∙s) ∙ (bt_mcomp x t)
-    end.
-
-  Fact bt_mcomp_spec x t u : u ∊ bt_mcomp x t <-> exists k, k ∊ t /\ u ≈ x∙k.
-  Proof.
-    revert u; induction t as [ | s _ t Ht ]; intros u; simpl.
-    + rewrite btm_inv_0; split; try tauto.
-      intros (k & Hk & _); revert Hk; rewrite btm_inv_0; auto.
-    + rewrite btm_inv; split.
-      * intros [ H | H ].
-        - exists s; split; auto.
-        - rewrite Ht in H.
-          destruct H as (k & ? & ?).
-          exists k; split; auto.
-      * intros (k & H1 & H2); revert H1 H2.
-        rewrite btm_inv, Ht.
-        intros [H2|H2] H1; auto.
-        - left; apply bte_trans with (1 := H1); auto.
-        - right; exists k; auto.
-  Qed.
-
-  (** Powerset bti_inv x ⊆ s∙t <-> x ⊆ t \/ exists y, y ⊆ t /\ x ≈ s∙y *)
-
-  Fixpoint bt_pow t :=
-    match t with
-      | ε   => ε∙ε 
-      | x∙t => bt_pow t ∪ bt_mcomp x (bt_pow t)
-    end.
-
-  Fact bt_pow_spec t x : x ∊ bt_pow t <-> x ⊆ t.
-  Proof.
-    revert x; induction t as [ | s _ t Ht ]; intros x; simpl.
-    + rewrite btm_inv, btm_inv_0, bti_inv_0, bte_inv_0; tauto.
-    + rewrite bti_inv, bt_cup_spec, bt_mcomp_spec, Ht.
-      split; intros [ | (y & H) ]; auto; right; exists y; 
-        revert H; rewrite Ht; auto.
-  Qed.
-
-  Fact bt_pow_transitive t : bt_transitive t -> bt_transitive (bt_pow t).
-  Proof.
-    intros H x y H1.
-    do 2 rewrite bt_pow_spec.
-    intros H2 z Hz.
-    apply H2 in H1.
-    revert Hz H1; apply H.
-  Qed.
-
-  Fact bte_incl_equiv s t : s ≈ t <-> s ⊆ t /\ t ⊆ s.
-  Proof.
-    split.
-    + intros H; split; apply bte_bti; auto.
-    + intros []; apply bti_equiv; auto.
-  Qed.
-
-  Fact bte_ext s t : s ≈ t <-> forall x, x ∊ s <-> x ∊ t.
-  Proof.
-    rewrite bte_incl_equiv; firstorder.
+    revert x; induction s as [ | y s Hs ] using bt_rect'; intros x; simpl.
+    + rewrite btm_inv_0; tauto.
+    + rewrite btm_inv, btm_inv, Hs; tauto.
   Qed.
 
   Fact bt_cup_left s t : s ⊆ s ∪ t.
@@ -926,7 +782,7 @@ Section btree.
     + intros [] z; rewrite bt_cup_spec; intros []; auto.
   Qed.
 
-  Fact bt_sg_inv x y : x∙ε ≈ y∙ε <-> x ≈ y.
+  Fact bt_sg_inv x y : x⪧∅ ≈ y⪧∅ <-> x ≈ y.
   Proof.
     split; auto.
     rewrite bte_ext.
@@ -935,10 +791,213 @@ Section btree.
     apply proj1 in H; destruct H; try tauto; auto.
   Qed.
 
-  Fact bte_sym x y : x ≈ y <-> y ≈ x.
-  Proof. split; auto. Qed.
 
-  Fact bt_sg_db_inv a x y : a∙ε ≈ x∙y∙ε <-> a ≈ x /\ a ≈ y.
+   
+  (** We compute the transitive closure *)
+
+  Definition bt_transitive t := forall u v, u ∈ v -> v ∈ t -> u ∈ t.
+
+  Reserved Notation "↓ x" (at level 1).
+
+  Fixpoint bt_tc t := 
+    match t with 
+      | ∅   => ∅
+      | s⪧t => s⪧(↓s ∪ ↓t)
+    end
+  where "↓ t" := (bt_tc t).
+
+  Fact bt_tc_congr_l u v t : u ≈ v -> u ∈ ↓t -> v ∈ ↓t.
+  Proof.
+    revert u v; induction t using bt_rect'; simpl; intros ? ? ?; apply btm_congr_l; auto.
+  Qed.
+
+  Fact bt_tc_congr_r u s t : s ≈ t -> u ∈ ↓s <-> u ∈ ↓t.
+  Proof.
+    intros H; revert H u. 
+    induction 1 as [ | s t | r s t H1 IH1 H2 IH2 | s t | s t u 
+                   | s s' t t' H1 IH1 H2 IH2 ]; intros v; try tauto.
+    + symmetry; auto.
+    + rewrite IH1; auto.
+    + simpl; repeat (rewrite btm_inv || rewrite bt_cup_spec); tauto.
+    + simpl; repeat (rewrite btm_inv || rewrite bt_cup_spec); tauto.
+    + simpl; repeat (rewrite btm_inv || rewrite bt_cup_spec).
+      rewrite IH1, IH2; split; intros [ H | [] ]; auto; left.
+      * apply bte_trans with s; auto.
+      * apply bte_trans with s'; auto.
+  Qed.
+
+  (** The transitive closure is composed of the x st x ∈ ... ∈ t *)
+
+  Theorem bt_tc_spec t x : x ∈ ↓t <-> exists n, ∈-chain (S n) x t.
+  Proof.
+    revert x; induction t as [ | s Hs t Ht ]; intros x; simpl.
+    + rewrite btm_inv_0; split; try tauto.
+      intros (n & Hn).
+      apply chain_inv_S in Hn.
+      destruct Hn as (y & H1 & H2).
+      apply bt_chain_inv_0 in H2.
+      destruct H2 as (_ & ->).
+      apply bte_discr in H1; tauto.
+    + rewrite btm_inv, bt_cup_spec, Hs, Ht.
+      split.
+      * intros [ H | [ (n & H) | (n & H) ] ].
+        - exists 0.
+          constructor 2 with (s⪧t).
+          ++ apply btm_inv; auto.
+          ++ constructor.
+        - exists (S n).
+          apply chain_snoc with s; auto.
+        - exists n; apply btm_chain_comp; auto.
+      * intros (n & H).
+        apply chain_snoc_inv in H.
+        destruct H as (y & H1 & H2).
+        apply btm_inv in H2.
+        destruct H2 as [ H2 | H2 ].
+        - destruct n as [ | n ].
+          ++ apply chain_inv_0 in H1; subst; auto.
+          ++ right; left; exists n.
+             revert H1; apply btm_chain_congr_r; auto.
+        - right; right; exists n.
+          apply chain_snoc with y; auto.
+  Qed.
+
+  Fact bt_tc_incr t : t ⊆ ↓t.
+  Proof.
+    intro; induction t; simpl; auto.
+    rewrite btm_inv, btm_inv, bt_cup_spec; tauto.
+  Qed.
+
+  Fact bt_tc_mono s t : s ⊆ t -> ↓s ⊆ ↓t.
+  Proof.
+    intros H x.
+    do 2 rewrite bt_tc_spec.
+    intros (n & Hn).
+    apply chain_snoc_inv in Hn.
+    destruct Hn as (y & H1 & H2).
+    exists n; apply chain_snoc with y; auto.
+  Qed.
+
+  Hint Resolve bt_tc_incr bt_tc_mono.
+ 
+  Theorem bt_tc_trans t : bt_transitive ↓t.
+  Proof.
+    induction t as [ | s Hs t Ht ]; simpl; intros u v H1 H2.
+    + apply btm_inv_0 in H2; tauto.
+    + apply btm_inv in H2.
+      rewrite bt_cup_spec in H2.
+      rewrite btm_inv, bt_cup_spec.
+      destruct H2 as [ H2 | [ H2 | H2 ] ].
+      * right; left; apply bt_tc_congr_r with (1 := H2); auto.
+      * right; left; revert H2; apply Hs; auto.
+      * right; right; revert H2; apply Ht; auto.
+  Qed.
+
+  Hint Resolve bt_tc_trans.
+
+  Fact bt_trans_chain n x y t : bt_transitive t -> ∈-chain n x y -> y ∈ t -> x ∈ t. 
+  Proof.
+    intros Ht; induction 1 as [ | n x y z H1 H2 IH2 ]; auto.
+    intros H; apply Ht with (1 := H1); auto.
+  Qed.
+
+  Hint Resolve bt_trans_chain.
+
+  Fact bt_tc_idem t : ↓(↓t) ⊆ ↓t.
+  Proof.
+    intros x; rewrite bt_tc_spec.
+    intros (n & Hn).
+    apply chain_snoc_inv in Hn.
+    destruct Hn as (y & H1 & H2).
+    revert H1 H2.
+    apply bt_trans_chain; auto.
+  Qed.
+
+  (*  (** Is this really needed *)
+ 
+  Fixpoint bt_bcup x t :=
+    match t with
+      | ∅   => ∅ 
+      | s⪧t => (x⪧s) ∪ (bt_bcup x t)
+    end.
+
+  Fact bt_bcup_spec x t u : u ∈ bt_bcup x t <-> exists k, u ∈ x⪧k /\ k ∈ t.
+  Proof.
+    revert u; induction t as [ | s t Ht ] using bt_rect'; intros u; simpl.
+    + rewrite btm_inv_0; split; try tauto.
+      intros (k & _ & Hk); revert Hk; rewrite btm_inv_0; auto.
+    + rewrite btm_inv, bt_cup_spec; split.
+      * intros [ H | [ H | H ] ].
+        - exists s; split; auto.
+          apply btm_congr_l with x; auto.
+        - exists s; split; auto.
+        - rewrite Ht in H.
+          destruct H as (k & ? & ?).
+          exists k; split; auto.
+      * intros (k & H1 & H2); revert H1 H2.
+        rewrite btm_inv, btm_inv.
+        intros [H1|H1] [H2|H2]; auto.
+        - right; left; revert H1; apply btm_congr_r; auto.
+        - right; right; apply Ht; exists k.
+          rewrite btm_inv; auto.
+  Qed.
+
+  *)
+
+  Fixpoint bt_mcomp x t :=
+    match t with
+      | ∅   => ∅ 
+      | s⪧t => (x⪧s) ⪧ (bt_mcomp x t)
+    end.
+
+  Fact bt_mcomp_spec x t u : u ∈ bt_mcomp x t <-> exists k, k ∈ t /\ u ≈ x⪧k.
+  Proof.
+    revert u; induction t as [ | s t Ht ] using bt_rect'; intros u; simpl.
+    + rewrite btm_inv_0; split; try tauto.
+      intros (k & Hk & _); revert Hk; rewrite btm_inv_0; auto.
+    + rewrite btm_inv; split.
+      * intros [ H | H ].
+        - exists s; split; auto.
+        - rewrite Ht in H.
+          destruct H as (k & ? & ?).
+          exists k; split; auto.
+      * intros (k & H1 & H2); revert H1 H2.
+        rewrite btm_inv, Ht.
+        intros [H2|H2] H1; auto.
+        - left; apply bte_trans with (1 := H1); auto.
+        - right; exists k; auto.
+  Qed.
+
+  (** Powerset bti_inv x ⊆ s⪧t <-> x ⊆ t \/ exists y, y ⊆ t /\ x ≈ s⪧y *)
+
+  Fixpoint bt_pow t :=
+    match t with
+      | ∅   => ∅⪧∅ 
+      | x⪧t => bt_pow t ∪ bt_mcomp x (bt_pow t)
+    end.
+
+  Fact bt_pow_spec t x : x ∈ bt_pow t <-> x ⊆ t.
+  Proof.
+    revert x; induction t as [ | s t Ht ] using bt_rect'; intros x; simpl.
+    + rewrite btm_inv, btm_inv_0, bti_inv_0, bte_inv_0; tauto.
+    + rewrite bti_inv, bt_cup_spec, bt_mcomp_spec, Ht.
+      split; intros [ | (y & H) ]; auto; right; exists y; 
+        revert H; rewrite Ht; auto.
+  Qed.
+
+  (** Powerset of transitive is transitive *)
+
+  Fact bt_pow_transitive t : bt_transitive t -> bt_transitive (bt_pow t).
+  Proof.
+    intros H x y H1.
+    do 2 rewrite bt_pow_spec.
+    intros H2 z Hz.
+    apply H2 in H1.
+    revert Hz H1; apply H.
+  Qed.
+
+  (** We start workin with pairs *)
+
+  Fact bt_sg_db_inv a x y : a⪧∅ ≈ x⪧y⪧∅ <-> a ≈ x /\ a ≈ y.
   Proof.
     split.
     + intros H.
@@ -948,10 +1007,10 @@ Section btree.
       repeat rewrite btm_inv_0.
       intros [|[]] [|[]]; auto.
     + intros [].
-      apply bte_trans with (a∙a∙ε); auto.
+      apply bte_trans with (a⪧a⪧∅); auto.
   Qed.
 
-  Fact bt_db_inv a b x y : a∙b∙ε ≈ x∙y∙ε <-> a ≈ x /\ b ≈ x /\ x ≈ y
+  Fact bt_db_inv a b x y : a⪧b⪧∅ ≈ x⪧y⪧∅ <-> a ≈ x /\ b ≈ x /\ x ≈ y
                                           \/ a ≈ x /\ b ≈ y
                                           \/ a ≈ y /\ b ≈ x.
   Proof.
@@ -971,11 +1030,11 @@ Section btree.
 
   (** pairs   (x,y) = { {x},{x,y} } *)
 
-  Definition bt_pair s t := (s∙ε)∙(s∙t∙ε)∙ε.
+  Definition bt_pair s t := (s⪧∅)⪧(s⪧t⪧∅)⪧∅.
 
   Notation "⟬ s , t ⟭" := (bt_pair s t) (at level 1).
 
-  Fact bt_pair_spec x s t : x ∊ ⟬ s,t⟭ <-> x ≈ s∙ε \/ x ≈ s∙t∙ε.
+  Fact bt_pair_spec x s t : x ∈ ⟬ s,t⟭ <-> x ≈ s⪧∅ \/ x ≈ s⪧t⪧∅.
   Proof. 
     unfold bt_pair; repeat rewrite btm_inv.
     rewrite btm_inv_0; tauto. 
@@ -986,7 +1045,7 @@ Section btree.
     split.
     2: intros []; unfold bt_pair; auto.
     intros H; rewrite bte_ext in H.
-    assert (forall x, (x ≈ s∙ε \/ x ≈ s∙t∙ε) <-> (x ≈ s'∙ε \/ x ≈ s'∙t'∙ε)) as H'.
+    assert (forall x, (x ≈ s⪧∅ \/ x ≈ s⪧t⪧∅) <-> (x ≈ s'⪧∅ \/ x ≈ s'⪧t'⪧∅)) as H'.
     { intros x; generalize (H x); do 2 rewrite bt_pair_spec; tauto. }
     clear H; revert H'; intros H.
     generalize (proj1 (H _) (or_introl (in_bte_refl _))) 
@@ -994,7 +1053,7 @@ Section btree.
                (proj2 (H _) (or_introl (in_bte_refl _))) 
                (proj2 (H _) (or_intror (in_bte_refl _))).
     repeat rewrite bt_db_inv.
-    do 2 rewrite (bte_sym (_∙_∙_)).
+    do 2 rewrite (bte_sym (_⪧_⪧_)).
     repeat rewrite bt_sg_inv.
     repeat rewrite bt_sg_db_inv.
     intros.
@@ -1011,20 +1070,30 @@ Section btree.
 
   (** FOL encoding a triples belonging to a set *)
  
-  Fact bt_enc_equiv s t : s ≈ t <-> forall x, x ∊ s <-> x ∊ t.
+  Fact bt_enc_equiv s t : s ≈ t <-> forall x, x ∈ s <-> x ∈ t.
   Proof. apply bte_ext. Qed.
 
-  Fact bt_enc_sg s t : s ≈ t∙ε <-> forall x, x ∊ s <-> x ≈ t.
+  Fact bt_enc_empty s : s ≈ ∅ <-> forall x, ~ x ∈ s.
   Proof.
-    rewrite bte_ext.
-    apply forall_equiv; intros x.
+    rewrite bte_ext; apply forall_equiv; intros x.
+    rewrite btm_inv_0; tauto.
+  Qed.
+
+  Fact bt_enc_sg s t : s ≈ t⪧∅ <-> forall x, x ∈ s <-> x ≈ t.
+  Proof.
+    rewrite bte_ext; apply forall_equiv; intros x.
     rewrite btm_inv, btm_inv_0; tauto.
   Qed.
- 
-  Fact bt_enc_pair p s t : p ≈ ⟬s,t⟭  <-> (forall x, x ∊ p <-> x ≈ s∙ε \/ x ≈ s∙t∙ε).
+
+  Fact bt_enc_db u s t : u ≈ s⪧t⪧∅ <-> forall x, x ∈ u <-> x ≈ s \/ x ≈ t.
   Proof.
-    rewrite bte_ext.
-    apply forall_equiv; intros x.
+    rewrite bte_ext; apply forall_equiv; intros x.
+    rewrite btm_inv, btm_inv, btm_inv_0; tauto.
+  Qed.
+ 
+  Fact bt_enc_pair p s t : p ≈ ⟬s,t⟭  <-> (forall x, x ∈ p <-> x ≈ s⪧∅ \/ x ≈ s⪧t⪧∅).
+  Proof.
+    rewrite bte_ext; apply forall_equiv; intros x.
     rewrite bt_pair_spec; tauto.
   Qed.
 
@@ -1037,7 +1106,7 @@ Section btree.
       apply bt_pair_equiv; auto.
   Qed.
 
-  Fact bt_enc_rel3 a b c t : ⟬a,⟬b,c⟭⟭  ∊ t <-> exists p, p ≈ ⟬a,⟬b,c⟭⟭ /\ p ∊ t.
+  Fact bt_enc_rel3 a b c t : ⟬a,⟬b,c⟭⟭  ∈ t <-> exists p, p ≈ ⟬a,⟬b,c⟭⟭ /\ p ∈ t.
   Proof.
     split.
     + exists ⟬a,⟬b,c⟭⟭ ; auto.
@@ -1047,11 +1116,11 @@ Section btree.
 
   Fixpoint tuple (l : list bt) :=
     match l with 
-      | nil  => ε 
+      | nil  => ∅ 
       | x::l => ⟬x,tuple l⟭
     end.
 
-  Fact bt_enc_tuple_0 p : p ≈ tuple nil <-> p ≈ ε.
+  Fact bt_enc_tuple_0 p : p ≈ tuple nil <-> p ≈ ∅.
   Proof. simpl; tauto. Qed.
 
   Fact bt_enc_tuple p x l : p ≈ tuple (x::l) <-> exists a, p ≈ ⟬x,a⟭ /\ a ≈ tuple l.
@@ -1063,22 +1132,34 @@ Section btree.
       apply bt_pair_equiv; auto.
   Qed.
 
-  (** Now how to encode the model 
+  (** Now how to encode the model given by k-ary relation over a finite
+      set of cardinal n
 
       A finite set (pos n) and a k-ary relation R : (pos n)^k -> Prop
-      Find a transitive btree t such that pos n injects into t
-    
-      forall x, y in t, both {x} and {x,y} belong to P(t)
-      hence <x,y> belongs to P(P(t))
-      and <x1,...,xk> belongs to P^2k(t) for any x1,...,xk in t 
-      So P^2k(t) contains any k-ary tuple if the image of (pos n).
-      Hence X = P^{2k+1}(t) contains all unary relations over k-ary tuple
-      hence all the k-ary relations over t.
-
-      So we encode R into the transitive set X, we have a globally
-      existentially quantified X_R and we replace any 
       
-      R (v1,...,vk) by <x1,...,xk> in X_R 
+      1) Find a transitive btree t such that pos n injects into t
+         For this, it is enough that its depth is greater that n
+    
+      2) forall x, y in t, both {x} and {x,y} belong to P(t)
+         hence <x,y> belongs to P(P(t))
+
+      3) and <x1,...,xk> belongs to P^2k(t) for any x1,...,xk in t 
+         So P^2k(t) contains any k-ary tuple if the image of (pos n).
+        
+      4) Hence X = P^{2k+1}(t) contains all unary relations over k-ary 
+         tuple hence all the k-ary relations over t.
+
+      5) So we can encode R into the transitive set X = P^{2k+1}(t). 
+         
+      6) In the logic, we have a globally existentially quantified X_R 
+         and we replace any 
+      
+               R (v1,...,vk) by <x1,...,xk> in X_R
+
+         encoded according to the above description
+
+         Perhaps follow the H10 technique to establish FOL encodability 
+         into the Σ(0,2) signature
 
       *)
 
@@ -1086,27 +1167,47 @@ Section btree.
 
   Section HF_struct.
 
-    Fact HF_cntr s t : s∙s∙t ≈ s∙t.
+    (** this is not needed and relates to ITP 2016 *)
+
+    Fact HF_cntr s t : s⪧s⪧t ≈ s⪧t.
     Proof. auto. Qed.
 
-    Fact HF_comm s t u : s∙t∙u ≈ t∙s∙u. 
+    Fact HF_comm s t u : s⪧t⪧u ≈ t⪧s⪧u. 
     Proof. auto. Qed.
 
-    Fact HF_empty s t : s∙t ≉ ε. 
+    Fact HF_empty s t : s⪧t ≉ ∅. 
     Proof. apply bte_discr. Qed.
 
-    Fact HF_choice s t u : s∙t∙u ≈ t∙u -> s ≈ t \/ s∙u ≈ u.
+    Fact HF_choice s t u : s⪧t⪧u ≈ t⪧u -> s ≈ t \/ s⪧u ≈ u.
     Proof. apply btm_inv. Qed.
 
     Variable P : bt -> Type.
 
     Hypothesis (HP0 : forall s t, s ≈ t -> P s -> P t)
-               (HP1 : P ε)
-               (HP2 : forall s t, P s -> P t -> P (s∙t)).
+               (HP1 : P ∅)
+               (HP2 : forall s t, P s -> P t -> P (s⪧t)).
 
     Theorem HF_rect : forall t, P t.
     Proof. apply bt_rect; auto. Qed.
 
   End HF_struct.
+
+  Check btm_finite_t.
+  Print bt_transitive.
+  Check bt_tc_trans.
+  Check bt_pow_transitive.
+
+  Check bt_enc_equiv.
+  Check bt_enc_empty.
+  Check bt_enc_sg.
+  Check bt_enc_db.
+  Check bt_pair_equiv. 
+  Check bt_enc_pair.
+  Check bt_enc_triple.
+  Check bt_enc_rel3. 
+ 
+  Print tuple.
+  Check bt_enc_tuple_0.
+  Check bt_enc_tuple.
 
 End btree.
